bug.v
@@ -1,0 +1,20 @@
+Section Bug.
+
+Variable local_blocks: nat->nat->option nat. 
+
+Theorem thm: 
+    forall slot: nat, 
+    forall node1 node2: nat, 
+    forall block3 block4: nat,
+    forall x1 x2:nat,
+    (forall block1 block2: nat, 
+    local_blocks node1 slot = Some block1 -> 
+    local_blocks node2 slot = Some block2 -> 
+    block1 = block2) -> 
+    local_blocks node1 (S slot) = Some block3 ->
+    local_blocks node2 (S slot) = Some block4 ->
+    block3 = block4.
+    intros.
+    apply H with (block1:=x1) (block2:=x2).
+
+End Bug. 
